Added pk_enc_reverse_msg function to core

src/core/DY.Core.Bytes.fst
@@ -1707,6 +1707,46 @@ let pk_dec_enc key nonce msg =
   normalize_term_spec pk_enc;
   normalize_term_spec pk
 
+/// Ghost reverse function for predicates
+
+val pk_enc_reverse_msg: enc_msg:bytes -> GTot (option bytes)
+let pk_enc_reverse_msg enc_msg =
+  match enc_msg with
+  | PkEnc pk nonce msg -> Some msg
+  | _ -> None
+
+/// Encryption lemma for the ghost reverse function
+
+val pk_enc_reverse_msg_enc_lemma:
+  pk_prin:bytes -> nonce:bytes ->
+  msg:bytes -> enc:bytes ->
+  Lemma
+  (requires
+    enc == pk_enc pk_prin nonce msg
+  )
+  (ensures
+    pk_enc_reverse_msg enc == Some msg
+  )
+let pk_enc_reverse_msg_enc_lemma pk_prin nonce msg enc =
+  normalize_term_spec pk_enc;
+  ()
+
+/// Decryption lemma for the ghost reverse function
+
+val pk_enc_reverse_msg_dec_lemma:
+  sk_prin:bytes ->
+  enc:bytes -> msg:bytes ->
+  Lemma
+  (requires
+    pk_dec sk_prin enc == Some msg
+  )
+  (ensures 
+    pk_enc_reverse_msg enc == Some msg
+  )
+let pk_enc_reverse_msg_dec_lemma sk_prin enc msg = 
+  normalize_term_spec pk_dec;
+  ()
+
 /// Lemma for attacker knowledge theorem.
 
 val pk_preserves_publishability:
